imp_system/imp/ImpProofs.v
@@ -253,7 +253,7 @@ Section PROOFS.
       (interp_imp ge (triggerUB) le0 : itree _ (lenv * T)) = triggerUB.
   Proof using.
     unfold interp_imp, interp_ImpState, interp_GlobEnv, LModTr.pure_state, triggerUB, trivial_Handler.
-    grind. rewrite interp_trigger. grind.
+    grind.
   Qed.
 
   Lemma interp_imp_triggerUB_bind
@@ -262,7 +262,7 @@ Section PROOFS.
       (interp_imp ge (x <- triggerUB;; ktr x) le0 : itree _ (lenv *T)) = triggerUB.
   Proof using.
     unfold interp_imp, interp_ImpState, interp_GlobEnv, LModTr.pure_state, triggerUB, trivial_Handler.
-    grind. rewrite interp_trigger. grind.
+    grind.
   Qed.
 
   Lemma interp_imp_triggerNB
@@ -271,7 +271,7 @@ Section PROOFS.
       (interp_imp ge (triggerNB) le0 : itree _ (lenv * T)) = triggerNB.
   Proof using.
     unfold interp_imp, interp_ImpState, interp_GlobEnv, LModTr.pure_state, triggerNB, trivial_Handler.
-    grind. rewrite interp_trigger. grind.
+    grind.
   Qed.
 
   Lemma interp_imp_triggerNB_bind
@@ -280,7 +280,7 @@ Section PROOFS.
       (interp_imp ge (x <- triggerNB;; ktr x) le0 : itree _ (lenv * T)) = triggerNB.
   Proof using.
     unfold interp_imp, interp_ImpState, interp_GlobEnv, LModTr.pure_state, triggerNB, trivial_Handler.
-    grind. rewrite interp_trigger. grind.
+    grind.
   Qed.
 
   Lemma interp_imp_unwrapU
@@ -315,9 +315,9 @@ Section PROOFS.
   Proof using.
     unfold interp_imp, interp_GlobEnv, interp_ImpState, unwrapU.
     des_ifs; grind.
-    - rewrite interp_trigger. grind.
+    - try rewrite interp_trigger. grind.
       unfold unwrapU. des_ifs. grind.
-    - rewrite interp_trigger. grind.
+    - try rewrite interp_trigger. grind.
       unfold unwrapU. des_ifs. unfold triggerUB, LModTr.pure_state. grind.
   Qed.
 
@@ -334,7 +334,7 @@ Section PROOFS.
     unfold interp_imp, interp_GlobEnv, interp_ImpState.
     destruct x as [?|[blk ofs]|]; try destruct ofs.
     1,3,4,5:(rewrite interp_trigger; grind; unfold triggerUB, LModTr.pure_state; grind).
-    rewrite interp_trigger. grind. unfold unwrapU.
+    try rewrite interp_trigger. grind. unfold unwrapU.
     destruct (CEnv.blk2id ge blk).
     { grind. }
     unfold triggerUB, LModTr.pure_state. grind.
@@ -347,7 +347,7 @@ Section PROOFS.
       r <- unwrapU (alist_find x le0);; tau;; tau;; Ret (le0, r).
   Proof using.
     unfold interp_imp, interp_ImpState, interp_GlobEnv, trivial_Handler.
-    rewrite interp_trigger. grind.
+    try rewrite interp_trigger. grind.
   Qed.
 
   Lemma interp_imp_SetVar
@@ -357,7 +357,7 @@ Section PROOFS.
       tau;; tau;; Ret (alist_add x v le0, ()).
   Proof using.
     unfold interp_imp, interp_GlobEnv, interp_ImpState, trivial_Handler.
-    rewrite interp_trigger. grind.
+    try rewrite interp_trigger. grind.
   Qed.
 
   Lemma interp_imp_ccallU
@@ -367,9 +367,8 @@ Section PROOFS.
       v <- trigger (Call f (args↑));; tau;; tau;; v <- (v↓)?;; Ret (le0, v).
   Proof using.
     unfold interp_imp, interp_GlobEnv, interp_ImpState, ccallU, trivial_Handler. grind.
-    unfold LModTr.pure_state. rewrite interp_trigger. grind.
-    unfold unwrapU. des_ifs; grind. unfold triggerUB. grind.
-    rewrite interp_trigger. grind.
+    unfold LModTr.pure_state. try rewrite interp_trigger. grind.
+    unfold unwrapU. des_ifs; grind.
   Qed.
 
   Lemma interp_imp_IO
@@ -379,7 +378,7 @@ Section PROOFS.
       v <- trigger (IO f args);; tau;; tau;; Ret (le0, (v : O)).
   Proof using.
     unfold interp_imp, interp_GlobEnv, interp_ImpState, trivial_Handler.
-    unfold LModTr.pure_state. rewrite interp_trigger. grind.
+    unfold LModTr.pure_state. try rewrite interp_trigger. grind.
   Qed.
 
   Lemma interp_imp_assume
@@ -388,7 +387,7 @@ Section PROOFS.
       interp_imp ge (assume p) le0 = assume p;;; tau;; tau;; Ret (le0, ()).
   Proof using.
     unfold interp_imp, interp_GlobEnv, interp_ImpState, trivial_Handler.
-    unfold assume. grind. rewrite interp_trigger. grind.
+    unfold assume. grind. try rewrite interp_trigger. grind.
     unfold LModTr.pure_state. grind.
   Qed.
 
@@ -398,7 +397,7 @@ Section PROOFS.
       interp_imp ge (guarantee p) le0 = guarantee p;;; tau;; tau;; Ret (le0, ()).
   Proof using.
     unfold interp_imp, interp_GlobEnv, interp_ImpState, trivial_Handler.
-    unfold guarantee. grind. rewrite interp_trigger. grind.
+    unfold guarantee. grind. try rewrite interp_trigger. grind.
     unfold LModTr.pure_state. grind.
   Qed.
 
