imp_system/mem/MemTactics.v
@@ -18,7 +18,7 @@ Section mem.
 
   Context (sp : specmap).
 
-  Lemma wsim_mem_alloc (sz : Z) (msk : emask) k_s k_t E1 E2 r g :
+  Lemma wsim_mem_alloc (sz : Z) (msk : emask) k_s k_t E1 E2 g :
     fl_t !! (fid MemHdr.alloc) =
       Some (Some (SB.sandbox_body
         (msk, SModTr.trans_fnsem sp (fsp_some MemA.alloc, fbody_trivial)))) →
@@ -26,10 +26,10 @@ Section mem.
     (0 <= 8 * sz < modulus_64)%Z →
     (∀ blk,
       ([∗ list] i ↦ v ∈ replicate (Z.to_nat sz) Vundef, (blk, Z.of_nat i)%Z ↦ v) -∗
-      wsim fl_s fl_t Ist (E1, E2) r g R_s R_t RR ps true
+      wsim fl_s fl_t Ist (E1, E2) g R_s R_t RR ps true
       (st_src, k_s)
       (st_tgt, k_t (Vptr (blk, 0%Z))↑)) ⊢
-    wsim fl_s fl_t Ist (E1, E2) r g R_s R_t RR ps pt
+    wsim fl_s fl_t Ist (E1, E2) g R_s R_t RR ps pt
       (st_src, k_s)
       (st_tgt, x <- (trigger (Call MemHdr.alloc.1 [Vint sz]↑));; k_t x).
   Proof using.
@@ -45,16 +45,16 @@ Section mem.
     iIntros "!> % % %"; rewrite Z.add_0_l; iIntros "$".
   Qed.
 
-  Lemma wsim_mem_free b ofs v' (msk : emask) k_s k_t E1 E2 r g :
+  Lemma wsim_mem_free b ofs v' (msk : emask) k_s k_t E1 E2 g :
     fl_t !! fid MemHdr.free =
       Some (Some (SB.sandbox_body
         (msk, SModTr.trans_fnsem sp (fsp_some MemA.free, fbody_trivial)))) →
     img_msk msk →
     (b, ofs) ↦ v' -∗
-    (wsim fl_s fl_t Ist (E1, E2) r g R_s R_t RR ps true
+    (wsim fl_s fl_t Ist (E1, E2) g R_s R_t RR ps true
         (st_src, k_s)
         (st_tgt, k_t (Vint 0)↑)) -∗
-    wsim fl_s fl_t Ist (E1, E2) r g R_s R_t RR ps pt
+    wsim fl_s fl_t Ist (E1, E2) g R_s R_t RR ps pt
       (st_src, k_s)
       (st_tgt, x <- trigger (Call MemHdr.free.1 [Vptr (b, ofs)]↑);; k_t x).
   Proof using.
@@ -66,17 +66,17 @@ Section mem.
     iDestruct "GRT" as "[-> ->]". iApply "K"; iFrame.
   Qed.
 
-  Lemma wsim_mem_store b ofs v v' (msk : emask) k_s k_t E1 E2 r g :
+  Lemma wsim_mem_store b ofs v v' (msk : emask) k_s k_t E1 E2 g :
     fl_t !! fid MemHdr.store =
       Some (Some (SB.sandbox_body
         (msk, SModTr.trans_fnsem sp (fsp_some MemA.store, fbody_trivial)))) →
     img_msk msk →
     (b, ofs) ↦ v' -∗
     ((b, ofs) ↦ v -∗
-      wsim fl_s fl_t Ist (E1, E2) r g R_s R_t RR ps true
+      wsim fl_s fl_t Ist (E1, E2) g R_s R_t RR ps true
         (st_src, k_s)
         (st_tgt, k_t (Vint 0)↑)) -∗
-    wsim fl_s fl_t Ist (E1, E2) r g R_s R_t RR ps pt
+    wsim fl_s fl_t Ist (E1, E2) g R_s R_t RR ps pt
       (st_src, k_s)
       (st_tgt, x <- trigger (Call MemHdr.store.1 [Vptr (b, ofs); v]↑);; k_t x).
   Proof using.
@@ -88,17 +88,17 @@ Section mem.
     iDestruct "GRT" as "[-> [↦ ->]]". iApply "K"; iFrame.
   Qed.
 
-  Lemma wsim_mem_load b ofs q v (msk : emask) k_s k_t E1 E2 r g :
+  Lemma wsim_mem_load b ofs q v (msk : emask) k_s k_t E1 E2 g :
      fl_t !! fid MemHdr.load =
       Some (Some (SB.sandbox_body
         (msk, SModTr.trans_fnsem sp (fsp_some MemA.load, fbody_trivial)))) →
     img_msk msk →
     (b, ofs) ↦{q} v -∗
     ((b, ofs) ↦{q} v -∗
-      wsim fl_s fl_t Ist (E1, E2) r g R_s R_t RR ps true
+      wsim fl_s fl_t Ist (E1, E2) g R_s R_t RR ps true
         (st_src, k_s)
         (st_tgt, k_t v↑)) -∗
-    wsim fl_s fl_t Ist (E1, E2) r g R_s R_t RR ps pt
+    wsim fl_s fl_t Ist (E1, E2) g R_s R_t RR ps pt
       (st_src, k_s)
       (st_tgt, x <- trigger (Call MemHdr.load.1 [Vptr (b, ofs)]↑);; k_t x).
   Proof using.
@@ -110,7 +110,7 @@ Section mem.
     iDestruct "GRT" as "[-> [↦ ->]]". iApply "K"; iFrame.
   Qed.
 
-  Lemma wsim_mem_cas b ofs v v_old v_new succ E (msk : emask) k_s k_t E1 E2 r g  :
+  Lemma wsim_mem_cas b ofs v v_old v_new succ E (msk : emask) k_s k_t E1 E2 g  :
     fl_t !! fid MemHdr.cas =
       Some (Some (SB.sandbox_body
         (msk, SModTr.trans_fnsem sp (fsp_some MemA.cas, fbody_trivial)))) →
@@ -122,10 +122,10 @@ Section mem.
           (MemA.val_r v q0 v0 ∗ MemA.val_r v_old q1 v1 ==∗ E)) -∗
     (((b, ofs) ↦ if (bool_decide (succ = 1)) then v_new else v) -∗
      E -∗
-      wsim fl_s fl_t Ist (E1, E2) r g R_s R_t RR ps true
+      wsim fl_s fl_t Ist (E1, E2) g R_s R_t RR ps true
         (st_src, k_s)
         (st_tgt, k_t v↑)) -∗
-    wsim fl_s fl_t Ist (E1, E2) r g R_s R_t RR ps pt
+    wsim fl_s fl_t Ist (E1, E2) g R_s R_t RR ps pt
       (st_src, k_s)
       (st_tgt, x <- trigger (Call MemHdr.cas.1 [Vptr (b, ofs); v_old; v_new]↑);; k_t x).
   Proof using.
@@ -138,7 +138,7 @@ Section mem.
     rewrite Hg; cStepsT. iDestruct "GRT" as "[-> [-> [↦ E]]]". iApply ("K" with "↦ E"); iFrame.
   Qed.
 
-  Lemma wsim_mem_cmp v1 v2 succ E (msk : emask) k_s k_t E1 E2 r g :
+  Lemma wsim_mem_cmp v1 v2 succ E (msk : emask) k_s k_t E1 E2 g :
     fl_t !! (fid MemHdr.cmp) =
       Some (Some (SB.sandbox_body
         (msk, SModTr.trans_fnsem sp (fsp_some (MemA.cmp), fbody_trivial)))) →
@@ -148,10 +148,10 @@ Section mem.
     (E ==∗ ∃ q0 q1 v1' v2', MemA.val_r v1 q0 v1' ∗ MemA.val_r v2 q1 v2' ∗
           (MemA.val_r v1 q0 v1' ∗ MemA.val_r v2 q1 v2' ==∗ E)) -∗
     (E -∗
-      wsim fl_s fl_t Ist (E1, E2) r g R_s R_t RR ps true
+      wsim fl_s fl_t Ist (E1, E2) g R_s R_t RR ps true
         (st_src, k_s)
         (st_tgt, k_t (Vint succ)↑)) -∗
-    wsim fl_s fl_t Ist (E1, E2) r g R_s R_t RR ps pt
+    wsim fl_s fl_t Ist (E1, E2) g R_s R_t RR ps pt
       (st_src, k_s)
       (st_tgt,
         x <- trigger (Call MemHdr.cmp.1 [v1; v2]↑);;
@@ -166,15 +166,15 @@ Section mem.
     iDestruct "GRT" as "[-> [-> E]]". iApply ("K" with "E"); iFrame.
   Qed.
 
-  Lemma wsim_mem_cmp_int n1 n2 (msk : emask) k_s k_t E1 E2 r g :
+  Lemma wsim_mem_cmp_int n1 n2 (msk : emask) k_s k_t E1 E2 g :
     fl_t !! (fid MemHdr.cmp) =
       Some (Some (SB.sandbox_body
         (msk, SModTr.trans_fnsem sp (fsp_some (MemA.cmp), fbody_trivial)))) →
     img_msk msk →
-    (wsim fl_s fl_t Ist (E1, E2) r g R_s R_t RR ps true
+    (wsim fl_s fl_t Ist (E1, E2) g R_s R_t RR ps true
         (st_src, k_s)
         (st_tgt, k_t (Vint (if decide (n1 = n2) then 1 else 0)%Z)↑)) -∗
-    wsim fl_s fl_t Ist (E1, E2) r g R_s R_t RR ps pt
+    wsim fl_s fl_t Ist (E1, E2) g R_s R_t RR ps pt
       (st_src, k_s)
       (st_tgt,
         x <- trigger (Call MemHdr.cmp.1 [Vint n1; Vint n2]↑);;
